Add `__mem_type` to GoContext to map typeIds to the underlying mem_type
(mem_type = go_type). This will help generatedproof write trusted
assumptions like `(∀ T_id, __functions ("someFunc[" + T_id + "]")
= someFuncⁱᵐᵖˡ T_id (__mem_type T_id))`. generatedproof can assemble
these assumptions in a record in universe Prop to help access them
efficiently (experiments with having a raw prop that's a conjunction of
a bunch of stuff was a little sketchy).

new/golang/defn/pkg.v
@@ -4,8 +4,8 @@ From Perennial Require Import base.
 (** [PkgInfo] associates a pkg_name to its static information. *)
 Class PkgInfo (pkg_name: go_string) `{ffi_syntax} := {
     pkg_vars : list (go_string * go_type);
-    pkg_functions : go_string → val → bool;
-    pkg_msets : go_string → list (go_string * val) → bool;
+    pkg_functions : go_string → option val;
+    pkg_msets : go_string → option (list (go_string * val));
     pkg_imported_pkgs : list go_string;
   }.
 
